
\renewcommand{\theequation}{\theenumi}
\begin{enumerate}[label=\thesection.\arabic*.,ref=\thesection.\theenumi]
\numberwithin{equation}{enumi}
	
\item To Prove EFGH is a cyclic quadrilateral, we have to show that the sum of one pair of opposite side is $180^{\circ}$
\\
In $\triangle AEB$
\begin{enumerate}
\item $\phase{ABE} +\phase{BAE}+\phase{AEB}$ = $180^{\circ}$
\\
(Angle Sum Property of a triangle)
\item $\phase{AEB}$ = $180^{\circ}-\phase{ABE}-\phase{BAE}$
\item $\phase{AEB}$ = $180^{\circ}-\frac{1}{2}(\phase{B}+\phase{A})$
\label{eq:1}
\\
(Since BF bisects $\phase{B}$ and AH bisects $\phase{A}$)
\end{enumerate}
%
\item Now, lines AH and BF intersect, so
\begin{enumerate}
\item $\phase{FEH}$=$\phase{AEB}$(Vertically Opposite angles)
\item $\therefore \phase{FEH}$=$180^{\circ}-(\frac{\phase{B}}{2}+\frac{\phase{A}}{2})$(From \ref{eq:1})
\label{eq:2}
\end{enumerate}
%
\item Similarly we can prove that 
\\
\label{eq:3}
$\phase{FGH}$=$180^{\circ}-(\frac{\phase{C}}{2}+\frac{\phase{D}}{2})$
\item Adding \eqref{eq:2} and \eqref{eq:3}
\begin{enumerate}
\item $\phase{FEH} + \phase{FGH}$=$180^{\circ}-(\frac{\phase{A}}{2}+\frac{\phase{D}}{2}+180^{\circ}-(\frac{\phase{C}}{2}+\frac{\phase{B}}{2})$
\item $\phase{FEH} + \phase{FGH}$=$360^{\circ}-\frac{1}{2}(\phase{A}+\phase{B}+\phase{C}+\phase{D})$
\\
(Since ABCD is a quadrilateral, Sum of angles in it = $360^{\circ}$)
\item $\phase{FEH} + \phase{FGH}$=$360^{\circ}-\frac{1}{2}(360^{\circ})$
\item $\phase{FEH} + \phase{FGH}$=$180^{\circ}$
\end{enumerate}
\item Thus in EFGH, since the sum of one pair of opposite angles is $180^{\circ}$.
\\
$\therefore$ EFGH is a cyclic quadrilateral.
\end{enumerate}