
From the figure, lets assume $\vec{C}$ to be the origin.
\newline
\begin{figure}[H]
\input{./figs/triangleABC.tex}
\caption{$\triangle ACB$}
\end{figure}
$\vec{C}=0$
\newline
$\vec{CA}=b\hat{j}$
\newline
$\vec{CB}=a\hat{i}$
\newline
$\vec{M}$ is the position vector of mid-point of $\vec{BA}$.
\newline
$\vec{CM} = \vec{CB}+\vec{BM}$ [$\vec{BM}=(1/2)*\vec{BA}$]
\newline
$\vec{CM} = a\hat{i}+(1/2)(b\hat{j}-a\hat{i})$
\newline
Therefore, $\vec{CM}=(1/2)(b\hat{j}+a\hat{i})$
\newline
\begin{figure}[H]
\input{./figs/triangleDBC.tex}
\caption{$\triangle DBC$}
\end{figure}
From the figure, $\vec{CD}=2(\vec{CM})$
\newline
$\vec{CD}=a\hat{i}+b\hat{j}$
